Given_Clause_Loops/Otter_Loop_Fairness.thy
@@ -2,36 +2,25 @@ theory Otter_Loop_Fairness
   imports Otter_Loop Loop_Fairness_Basis
 begin
 
-type_synonym ('p, 'f) fair_OL_state = "'p \<times> 'f set \<times> 'f set \<times> 'f set \<times> 'f set"
+type_synonym ('p, 'f) fair_OL_state = "'f set \<times> 'f set \<times> 'p \<times> 'f set \<times> 'f set"
 
-datatype otter_loop_label =
+datatype OL_label =
   Active | New | XX | Passive | YY
 
-fun Prec_L :: "otter_loop_label \<Rightarrow> otter_loop_label \<Rightarrow> bool" where
-  "Prec_L YY _ \<longleftrightarrow> False"
-| "Prec_L Passive YY \<longleftrightarrow> True"
-| "Prec_L Passive _ \<longleftrightarrow> False"
-| "Prec_L XX YY \<longleftrightarrow> True"
-| "Prec_L XX Passive \<longleftrightarrow> True"
-| "Prec_L XX _ \<longleftrightarrow> False"
-| "Prec_L New YY \<longleftrightarrow> True"
-| "Prec_L New Passive \<longleftrightarrow> True"
-| "Prec_L New XX \<longleftrightarrow> True"
-| "Prec_L New _ \<longleftrightarrow> False"
-| "Prec_L Active YY \<longleftrightarrow> True"
-| "Prec_L Active Passive \<longleftrightarrow> True"
-| "Prec_L Active XX \<longleftrightarrow> True"
-| "Prec_L Active New \<longleftrightarrow> True"
-| "Prec_L Active Active \<longleftrightarrow> False"
+primrec nat_of_OL_label :: "OL_label \<Rightarrow> nat" where
+  "nat_of_OL_label Active = 0"
+| "nat_of_OL_label New = 1"
+| "nat_of_OL_label XX = 2"
+| "nat_of_OL_label Passive = 3"
+| "nat_of_OL_label YY = 4"
 
-(*
-"('f \<times> otter_loop_label) inference set"
-*)
+definition OL_Prec_L :: "OL_label \<Rightarrow> OL_label \<Rightarrow> bool" where
+  "OL_Prec_L l l' \<longleftrightarrow> nat_of_OL_label l < nat_of_OL_label l'"
 
 locale fair_otter_loop =
-  ol: otter_loop Bot_F Inf_F Bot_G Q entails_q Inf_G_q Red_I_q Red_F_q \<G>_F_q \<G>_I_q Inf_FL Equiv_F
-    Prec_F Prec_L Active New XX Passive YY +
-  ps: passive_struct
+  otter_loop Bot_F Inf_F Bot_G Q entails_q Inf_G_q Red_I_q Red_F_q \<G>_F_q \<G>_I_q Equiv_F Prec_F
+    OL_Prec_L Active New XX Passive YY +
+  ps: passive_set empty select add fformulas
   for
     Bot_F :: "'f set" and
     Inf_F :: "'f inference set" and
@@ -43,22 +32,28 @@ locale fair_otter_loop =
     Red_F_q :: "'q \<Rightarrow> 'g set \<Rightarrow> 'g set" and
     \<G>_F_q :: "'q \<Rightarrow> 'f \<Rightarrow> 'g set" and
     \<G>_I_q :: "'q \<Rightarrow> 'f inference \<Rightarrow> 'g inference set option" and
-    Inf_F :: "'f inference set" and
     Equiv_F :: "'f \<Rightarrow> 'f \<Rightarrow> bool" (infix \<open>\<doteq>\<close> 50) and
-    Prec_F :: "'f \<Rightarrow> 'f \<Rightarrow> bool" (infix \<open>\<prec>\<cdot>\<close> 50)
+    Prec_F :: "'f \<Rightarrow> 'f \<Rightarrow> bool" (infix \<open>\<prec>\<cdot>\<close> 50) and
+    empty :: "'p" and
+    select :: "'p \<Rightarrow> 'f \<times> 'p" and
+    add :: "'f list \<Rightarrow> 'p \<Rightarrow> 'p" and
+    fformulas :: "'p \<Rightarrow> 'f fset"
 begin
 
-inductive fair_OL :: "('f \<times> 'l) set \<Rightarrow> ('f \<times> 'l) set \<Rightarrow> bool" (infix "\<leadsto>OLf" 50) where
-  choose_n: "C \<notin> N \<Longrightarrow> state (N \<union> {C}, {}, P, {}, A) \<leadsto>OLf state (N, {C}, P, {}, A) "
-| delete_fwd: "C \<in> no_labels.Red_F (P \<union> A) \<or> (\<exists>C'\<in> (P \<union> A). C' \<preceq>\<cdot> C) \<Longrightarrow>
-    state (N, {C}, P, {}, A) \<leadsto>OLf state (N, {}, P, {}, A) "
-| simplify_fwd: "C \<in> no_labels.Red_F (P \<union> A \<union> {C'}) \<Longrightarrow>
-    state (N, {C}, P, {}, A) \<leadsto>OLf state (N, {C'}, P, {}, A)"
-| delete_bwd_p: "C' \<in> no_labels.Red_F ({C}) \<or> C \<prec>\<cdot> C'  \<Longrightarrow>
-    state (N, {C}, P \<union> {C'}, {}, A) \<leadsto>OLf state(N, {C}, P, {}, A)"
+inductive
+  fair_OL :: "('p, 'f) fair_OL_state \<Rightarrow> ('p, 'f) fair_OL_state \<Rightarrow> bool" (infix "\<leadsto>OLf" 50)
+where
+  choose_n: "C \<notin> N \<Longrightarrow> (N \<union> {C}, {}, P, {}, A) \<leadsto>OLf (N, {C}, P, {}, A)"
+| delete_fwd: "C \<in> no_labels.Red_F (formulas P \<union> A) \<or> (\<exists>C' \<in> formulas P \<union> A. C' \<preceq>\<cdot> C) \<Longrightarrow>
+    (N, {C}, P, {}, A) \<leadsto>OLf (N, {}, P, {}, A)"
+| simplify_fwd: "C \<in> no_labels.Red_F (formulas P \<union> A \<union> {C'}) \<Longrightarrow>
+    (N, {C}, P, {}, A) \<leadsto>OLf (N, {C'}, P, {}, A)"
+| delete_bwd_p: "C' \<in> formulas P \<Longrightarrow> C' \<in> no_labels.Red_F {C} \<or> C \<prec>\<cdot> C' \<Longrightarrow>
+    (N, {C}, P, {}, A) \<leadsto>OLf (N, {C}, delete C' P, {}, A)"
+(*
 | simplify_bwd_p: "C' \<in> no_labels.Red_F ({C, C''}) \<Longrightarrow>
     state (N, {C}, P \<union> {C'}, {}, A) \<leadsto>OLf state (N \<union> {C''}, {C}, P, {}, A)"
-| delete_bwd_a: "C' \<in> no_labels.Red_F ({C}) \<or> C \<prec>\<cdot> C'  \<Longrightarrow>
+| delete_bwd_a: "C' \<in> no_labels.Red_F {C} \<or> C \<prec>\<cdot> C' \<Longrightarrow>
     state (N, {C}, P, {}, A \<union> {C'}) \<leadsto>OLf state (N, {C}, P, {}, A)"
 | simplify_bwd_a: "C' \<in> no_labels.Red_F ({C, C'' }) \<Longrightarrow>
     state (N, {C}, P, {}, A \<union> {C'}) \<leadsto>OLf state (N \<union> {C''}, {C}, P, {}, A)"
@@ -66,7 +61,7 @@ inductive fair_OL :: "('f \<times> 'l) set \<Rightarrow> ('f \<times> 'l) set \<
 | choose_p: "C \<notin> P \<Longrightarrow> state ({}, {}, P \<union> {C}, {}, A) \<leadsto>OLf state ({}, {}, P, {C}, A)"
 | infer: "no_labels.Inf_between A {C} \<subseteq> no_labels.Red_I (A \<union> {C} \<union> M) \<Longrightarrow>
     state ({}, {}, P, {C}, A) \<leadsto>OLf state  (M, {}, P, {}, A \<union> {C})"
-
+*)
 
 
 thm gc_fair
